txn-data-consistency/Prot_2PC_2PL.thy
@@ -8,21 +8,22 @@ subsection \<open>2PC Event system\<close>
 
 subsubsection \<open>State\<close>
 
-datatype status_rm = working | prepared | okay | notokay | committed | aborted |
-                     prep_uabort | user_aborted
-datatype status_tm = tm_init | tm_prepared | tm_committed | tm_aborted | tm_user_aborted
+datatype status_rm = working | prepared | okay | notokay | committed | aborted
+datatype status_tm = tm_init | tm_prepared | tm_committed | tm_aborted
 
 record tm_state =
   tm_status :: status_tm
-  tm_tid :: nat
+  tm_tid :: txid0
+  tm_view :: view
 
 typedecl rmid
+consts loc :: "key \<Rightarrow> rmid"
 
 record 'v rm_state =
-  rm_main_db :: "'v kv_store"
-  rm_shadow_db :: "'v kv_store"
+  rm_db :: "'v kv_store"
+  rm_fingerpr :: "'v fingerpr"
   rm_status :: status_rm
-  rm_tid :: nat
+  rm_tid :: txid0
 
 type_synonym 'v rms_state = "rmid \<Rightarrow> 'v rm_state"
 
@@ -33,10 +34,166 @@ record 'v global_state =
 
 subsubsection \<open>Events\<close>
 
-datatype ev2 = Prepare rmid | OK rmid | NOK rmid | PrepUAbort rmid |
-               UAbort rmid | Commit rmid | Abort rmid | Ready rmid |
-               User_Commit | User_Abort | TM_Commit | TM_Abort |
-               TM_ReadyC | TM_ReadyA | Skip
+datatype 'v ev = Write2 rmid key 'v | Read2 rmid key 'v |
+                 Prepare rmid | OK rmid | NOK rmid | Commit rmid | Abort rmid | Ready rmid |
+                 User_Commit | TM_Commit | TM_Abort | TM_ReadyC | TM_ReadyA | TM_Skip
+
+definition other_rms_unchanged where
+  "other_rms_unchanged rm rmss rmss' \<equiv> (\<forall>rm'. rm' \<noteq> rm \<longrightarrow> rmss' rm' = rmss rm')"
+
+abbreviation tm_other_rms_unchanged where
+  "tm_other_rms_unchanged rm s s' \<equiv> tm s' = tm s \<and> other_rms_unchanged rm (rms s) (rms s')"
+
+abbreviation tid_match where
+  "tid_match s rm \<equiv> rm_tid (rms s rm) = tm_tid (tm s)"
+
+abbreviation rm_status_trans where
+  "rm_status_trans s rm s' from_stat to_stat \<equiv>
+      rm_status (rms s rm) = from_stat
+    \<and> rm_db (rms s' rm) = rm_db (rms s rm)
+    \<and> rm_fingerpr (rms s' rm) = rm_fingerpr (rms s rm)
+    \<and> rm_status (rms s' rm) = to_stat
+    \<and> rm_tid (rms s' rm) = rm_tid (rms s rm)
+    \<and> tm_other_rms_unchanged rm s s'"
+
+definition tid_inc :: "txid0"
+
+definition wriite where
+  "wriite s rm k v s' \<equiv> loc k = rm
+                        \<and> rm_status (rms s rm) = working
+                        \<and> tid_match s rm
+                        \<and> rm_fingerpr (rms s' rm) = update_fp (rm_fingerpr (rms s rm)) (Write k v)
+                        \<and> rm_status (rms s' rm) = working
+                        \<and> rm_db (rms s' rm) = rm_db (rms s rm)
+                        \<and> rm_tid (rms s' rm) = rm_tid (rms s rm)
+                        \<and> tm_other_rms_unchanged rm s s'"
+
+definition read where
+  "read s rm k v s' \<equiv> loc k = rm 
+                        \<and> rm_status (rms s rm) = working
+                        \<and> tid_match s rm
+                        \<and> rm_fingerpr (rms s' rm) = update_fp (rm_fingerpr (rms s rm)) (Read k v)
+                        \<comment> \<open>\<and> ov = (rm_main_db (rms s rm) ++ rm_shadow_db (rms s rm)) k\<close>
+                        \<and> rm_status (rms s' rm) = working
+                        \<and> rm_db (rms s' rm) = rm_db (rms s rm)
+                        \<and> rm_tid (rms s' rm) = rm_tid (rms s rm)
+                        \<and> tm_other_rms_unchanged rm s s'"
+
+definition prepare where
+  "prepare s rm s' \<equiv> tm_status (tm s) = tm_prepared
+                      \<and> rm_status_trans s rm s' working prepared"
+
+definition ok where \<comment>\<open>Lock acquired\<close>
+  "ok s rm s' \<equiv> tm_status (tm s) = tm_prepared
+                \<and> rm_status_trans s rm s' prepared okay"
+
+definition nok where \<comment>\<open>Lock not available\<close>
+  "nok s rm s' \<equiv> tm_status (tm s) = tm_prepared
+                \<and> rm_status_trans s rm s' prepared notokay"
+
+definition commit where
+  "commit s rm s' \<equiv> rm_status (rms s rm) = okay
+                    \<and> tm_status (tm s) = tm_committed
+                    \<and> rm_db (rms s' rm) =  update_kv (rm_tid (rms s rm)) (rm_fingerpr (rms s rm))
+                                                     (tm_view (tm s)) (rm_db (rms s rm)) \<comment>\<open>?\<close>
+                    \<and> rm_fingerpr (rms s' rm) = Map.empty
+                    \<and> rm_status (rms s' rm) = committed
+                    \<and> rm_tid (rms s' rm) = rm_tid (rms s rm)
+                    \<and> tm_other_rms_unchanged rm s s'"
+
+definition abort where \<comment>\<open>Lock released (if starting from okay)\<close>
+  "abort s rm s' \<equiv> (rm_status (rms s rm) = okay \<or>
+                    rm_status (rms s rm) = notokay)
+                    \<and> tm_status (tm s) = tm_aborted
+                    \<and> rm_db (rms s' rm) = rm_db (rms s rm)
+                    \<and> rm_fingerpr (rms s' rm) = Map.empty
+                    \<and> rm_status (rms s' rm) = aborted
+                    \<and> rm_tid (rms s' rm) = rm_tid (rms s rm)
+                    \<and> tm_other_rms_unchanged rm s s'"
+
+definition ready where \<comment>\<open>Lock released (if starting from committed)\<close>
+  "ready s rm s' \<equiv> ((rm_status (rms s rm) = committed \<and> tm_status (tm s) = tm_committed)
+                      \<or> (rm_status (rms s rm) = aborted \<and> tm_status (tm s) = tm_aborted))
+                   \<and> rm_status (rms s' rm) = working
+                   \<and> rm_tid (rms s' rm) = Suc (rm_tid (rms s rm))
+                   \<and> rm_db (rms s' rm) = rm_db (rms s rm)
+                   \<and> rm_fingerpr (rms s' rm) = rm_fingerpr (rms s rm)
+                   \<and> tm_other_rms_unchanged rm s s'"
+
+definition user_commit where
+  "user_commit s s' \<equiv> tm_status (tm s) = tm_init
+                      \<and> tm_status (tm s') = tm_prepared
+                      \<and> tm_tid (tm s') = tm_tid (tm s)
+                      \<and> tm_view (tm s') = tm_view (tm s)
+                      \<and> rms s' = rms s"
+
+definition tm_commit where
+  "tm_commit s s' \<equiv> tm_status (tm s) = tm_prepared
+                    \<and> (\<forall>rm. rm_status (rms s rm) = okay)
+                    \<and> tm_status (tm s') = tm_committed
+                    \<and> tm_tid (tm s') = tm_tid (tm s)
+                    \<and> tm_view (tm s') = tm_view (tm s)
+                    \<and> rms s' = rms s"
+
+definition tm_abort where
+  "tm_abort s s' \<equiv> (tm_status (tm s) = tm_prepared
+                     \<and> (\<exists>rm. rm_status (rms s rm) = notokay)
+                     \<and> (\<forall>rm. rm_status (rms s rm) = okay \<or> rm_status (rms s rm) = notokay))
+                    \<and> tm_status (tm s') = tm_aborted
+                    \<and> tm_tid (tm s') = tm_tid (tm s)
+                    \<and> tm_view (tm s') = tm_view (tm s)
+                    \<and> rms s' = rms s"
+
+definition tm_ready_c where
+  "tm_ready_c s s' \<equiv> tm_status (tm s) = tm_committed
+                    \<and> (\<forall>rm. rm_status (rms s rm) = working \<and> rm_tid (rms s rm) = Suc (tm_tid (tm s)))
+                    \<and> tm_status (tm s') = tm_init
+                    \<and> tm_tid (tm s') = Suc (tm_tid (tm s))
+                    \<and> tm_view (tm s') = tm_view (tm s) \<comment>\<open>Should see its own transaction?\<close>
+                    \<and> rms s' = rms s"
+
+definition tm_ready_a where
+  "tm_ready_a s s' \<equiv> tm_status (tm s) = tm_aborted
+                    \<and> (\<forall>rm. rm_status (rms s rm) = working \<and> rm_tid (rms s rm) = Suc (tm_tid (tm s)))
+                    \<and> tm_status (tm s') = tm_init
+                    \<and> tm_tid (tm s') = Suc (tm_tid (tm s))
+                    \<and> tm_view (tm s') = tm_view (tm s) \<comment>\<open>Should see its own transaction?\<close>
+                    \<and> rms s' = rms s"
+
+text\<open>The Event System\<close>
+definition gs_init :: "'v global_state" where
+  "gs_init \<equiv> \<lparr> 
+    tm = \<lparr> tm_status = tm_init, tm_tid = , tm_view = view_init \<rparr>,
+    rms = (\<lambda>rm. \<lparr> rm_db = kvs_init, rm_fingerpr = Map.empty, 
+                  rm_status = working, rm_tid = 0 \<rparr>)
+  \<rparr>"
+
+fun gs_trans :: "'v global_state \<Rightarrow> ev \<Rightarrow> 'v global_state \<Rightarrow> bool" where
+  "gs_trans s (Prepare rm)    s' \<longleftrightarrow> prepare s rm s'" |
+  "gs_trans s (OK rm)         s' \<longleftrightarrow> ok s rm s'" |
+  "gs_trans s (NOK rm)        s' \<longleftrightarrow> nok s rm s'" |
+  (*"gs_trans s (Commit rm)     s' \<longleftrightarrow> commit s rm s'" |*)
+  "gs_trans s (Abort rm)      s' \<longleftrightarrow> abort s rm s'" |
+  "gs_trans s (Ready rm)      s' \<longleftrightarrow> ready s rm s'" |
+  "gs_trans s User_Commit     s' \<longleftrightarrow> user_commit s s'" |
+  "gs_trans s TM_Commit       s' \<longleftrightarrow> tm_commit s s'" |
+  "gs_trans s TM_Abort        s' \<longleftrightarrow> tm_abort s s'" |
+  "gs_trans s TM_ReadyC       s' \<longleftrightarrow> tm_ready_c s s'" |
+  "gs_trans s TM_ReadyA       s' \<longleftrightarrow> tm_ready_a s s'" |
+  "gs_trans s TM_Skip         s' \<longleftrightarrow> s' = s"
+
+definition tps :: "(ev, 'v global_state) ES" where
+  "tps \<equiv> \<lparr>
+    init = (=) gs_init,
+    trans = gs_trans
+  \<rparr>"
+
+lemmas tps_trans_defs = prepare_def ok_def nok_def (*commit_def*) abort_def ready_def
+                        user_commit_def tm_commit_def tm_abort_def tm_ready_c_def tm_ready_a_def
+
+lemmas tps_defs = tps_def gs_init_def
+
+lemma tps_trans [simp]: "trans tps = gs_trans" by (simp add: tps_def)
 
 
 end
